# Functoriality of coproduct types

```agda
module foundation.functoriality-coproduct-types where
```

<details><summary>Imports</summary>

```agda
open import foundation.action-on-identifications-functions
open import foundation.coproduct-types
open import foundation.dependent-pair-types
open import foundation.equality-cartesian-product-types
open import foundation.equality-coproduct-types
open import foundation.equivalence-extensionality
open import foundation.equivalences
open import foundation.function-extensionality
open import foundation.functoriality-cartesian-product-types
open import foundation.homotopies
open import foundation.propositional-truncations
open import foundation.structure-identity-principle
open import foundation.surjective-maps
open import foundation.unit-type
open import foundation.universal-property-coproduct-types
open import foundation.universe-levels

open import foundation-core.cartesian-product-types
open import foundation-core.contractible-types
open import foundation-core.empty-types
open import foundation-core.fibers-of-maps
open import foundation-core.function-types
open import foundation-core.functoriality-dependent-function-types
open import foundation-core.functoriality-dependent-pair-types
open import foundation-core.identity-types
open import foundation-core.injective-maps
open import foundation-core.negation
open import foundation-core.propositions
open import foundation-core.transport
```

</details>

## Idea

Any two maps `f : A → B` and `g : C → D` induce a map
`map-coprod f g : coprod A B → coprod C D`.

## Definitions

### The functorial action of the coproduct operation

```agda
module _
  {l1 l2 l1' l2' : Level} {A : UU l1} {B : UU l2} {A' : UU l1'} {B' : UU l2'}
  where

  map-coprod : (A → A') → (B → B') → A + B → A' + B'
  map-coprod f g (inl x) = inl (f x)
  map-coprod f g (inr y) = inr (g y)
```

## Properties

### Functoriality of coproducts preserves identity maps

```agda
module _
  {l1 l2 : Level} (A : UU l1) (B : UU l2)
  where

  id-map-coprod : (map-coprod (id {A = A}) (id {A = B})) ~ id
  id-map-coprod (inl x) = refl
  id-map-coprod (inr x) = refl
```

### Functoriality of coproducts preserves composition

```agda
module _
  {l1 l2 l1' l2' l1'' l2'' : Level}
  {A : UU l1} {B : UU l2} {A' : UU l1'} {B' : UU l2'}
  {A'' : UU l1''} {B'' : UU l2''}
  (f : A → A') (f' : A' → A'') (g : B → B') (g' : B' → B'')
  where

  preserves-comp-map-coprod :
    (map-coprod (f' ∘ f) (g' ∘ g)) ~ ((map-coprod f' g') ∘ (map-coprod f g))
  preserves-comp-map-coprod (inl x) = refl
  preserves-comp-map-coprod (inr y) = refl
```

### Functoriality of coproducts preserves homotopies

```agda
module _
  {l1 l2 l1' l2' : Level} {A : UU l1} {B : UU l2} {A' : UU l1'} {B' : UU l2'}
  {f f' : A → A'} (H : f ~ f') {g g' : B → B'} (K : g ~ g')
  where

  htpy-map-coprod : (map-coprod f g) ~ (map-coprod f' g')
  htpy-map-coprod (inl x) = ap inl (H x)
  htpy-map-coprod (inr y) = ap inr (K y)
```

### The fibers of `map-coprod`

```agda
module _
  {l1 l2 l1' l2' : Level} {A : UU l1} {B : UU l2} {A' : UU l1'} {B' : UU l2'}
  (f : A' → A) (g : B' → B)
  where

  fib-map-coprod-inl-fib : (x : A) → fib f x → fib (map-coprod f g) (inl x)
  pr1 (fib-map-coprod-inl-fib x (pair a' p)) = inl a'
  pr2 (fib-map-coprod-inl-fib x (pair a' p)) = ap inl p

  fib-fib-map-coprod-inl : (x : A) → fib (map-coprod f g) (inl x) → fib f x
  fib-fib-map-coprod-inl x (pair (inl a') p) =
    pair a' (map-compute-eq-coprod-inl-inl (f a') x p)
  fib-fib-map-coprod-inl x (pair (inr b') p) =
    ex-falso (is-empty-eq-coprod-inr-inl (g b') x p)

  abstract
    is-section-fib-fib-map-coprod-inl :
      (x : A) → (fib-map-coprod-inl-fib x ∘ fib-fib-map-coprod-inl x) ~ id
    is-section-fib-fib-map-coprod-inl .(f a') (pair (inl a') refl) = refl
    is-section-fib-fib-map-coprod-inl x (pair (inr b') p) =
      ex-falso (is-empty-eq-coprod-inr-inl (g b') x p)

  abstract
    is-retraction-fib-fib-map-coprod-inl :
      (x : A) → (fib-fib-map-coprod-inl x ∘ fib-map-coprod-inl-fib x) ~ id
    is-retraction-fib-fib-map-coprod-inl .(f a') (pair a' refl) = refl

  abstract
    is-equiv-fib-map-coprod-inl-fib :
      (x : A) → is-equiv (fib-map-coprod-inl-fib x)
    is-equiv-fib-map-coprod-inl-fib x =
      is-equiv-has-inverse
        ( fib-fib-map-coprod-inl x)
        ( is-section-fib-fib-map-coprod-inl x)
        ( is-retraction-fib-fib-map-coprod-inl x)

  fib-map-coprod-inr-fib : (y : B) → fib g y → fib (map-coprod f g) (inr y)
  pr1 (fib-map-coprod-inr-fib y (pair b' p)) = inr b'
  pr2 (fib-map-coprod-inr-fib y (pair b' p)) = ap inr p

  fib-fib-map-coprod-inr : (y : B) → fib (map-coprod f g) (inr y) → fib g y
  fib-fib-map-coprod-inr y (pair (inl a') p) =
    ex-falso (is-empty-eq-coprod-inl-inr (f a') y p)
  pr1 (fib-fib-map-coprod-inr y (pair (inr b') p)) = b'
  pr2 (fib-fib-map-coprod-inr y (pair (inr b') p)) =
    map-compute-eq-coprod-inr-inr (g b') y p

  abstract
    is-section-fib-fib-map-coprod-inr :
      (y : B) → (fib-map-coprod-inr-fib y ∘ fib-fib-map-coprod-inr y) ~ id
    is-section-fib-fib-map-coprod-inr .(g b') (pair (inr b') refl) = refl
    is-section-fib-fib-map-coprod-inr y (pair (inl a') p) =
      ex-falso (is-empty-eq-coprod-inl-inr (f a') y p)

  abstract
    is-retraction-fib-fib-map-coprod-inr :
      (y : B) → (fib-fib-map-coprod-inr y ∘ fib-map-coprod-inr-fib y) ~ id
    is-retraction-fib-fib-map-coprod-inr .(g b') (pair b' refl) = refl

  abstract
    is-equiv-fib-map-coprod-inr-fib :
      (y : B) → is-equiv (fib-map-coprod-inr-fib y)
    is-equiv-fib-map-coprod-inr-fib y =
      is-equiv-has-inverse
        ( fib-fib-map-coprod-inr y)
        ( is-section-fib-fib-map-coprod-inr y)
        ( is-retraction-fib-fib-map-coprod-inr y)
```

### Functoriality of coproducts preserves equivalences

```agda
module _
  {l1 l2 l1' l2' : Level} {A : UU l1} {B : UU l2} {A' : UU l1'} {B' : UU l2'}
  where

  abstract
    is-equiv-map-coprod :
      {f : A → A'} {g : B → B'} →
      is-equiv f → is-equiv g → is-equiv (map-coprod f g)
    pr1
      ( pr1
        ( is-equiv-map-coprod
          ( pair (pair sf Sf) (pair rf Rf))
          ( pair (pair sg Sg) (pair rg Rg)))) = map-coprod sf sg
    pr2
      ( pr1
        ( is-equiv-map-coprod {f} {g}
          ( pair (pair sf Sf) (pair rf Rf))
          ( pair (pair sg Sg) (pair rg Rg)))) =
      ( ( inv-htpy (preserves-comp-map-coprod sf f sg g)) ∙h
        ( htpy-map-coprod Sf Sg)) ∙h
      ( id-map-coprod A' B')
    pr1
      ( pr2
        ( is-equiv-map-coprod
          ( pair (pair sf Sf) (pair rf Rf))
          ( pair (pair sg Sg) (pair rg Rg)))) = map-coprod rf rg
    pr2
      ( pr2
        ( is-equiv-map-coprod {f} {g}
          ( pair (pair sf Sf) (pair rf Rf))
          ( pair (pair sg Sg) (pair rg Rg)))) =
      ( ( inv-htpy (preserves-comp-map-coprod f rf g rg)) ∙h
        ( htpy-map-coprod Rf Rg)) ∙h
      ( id-map-coprod A B)

  map-equiv-coprod :
    (A ≃ A') → (B ≃ B') → A + B → A' + B'
  map-equiv-coprod e e' = map-coprod (map-equiv e) (map-equiv e')

  equiv-coprod :
    (A ≃ A') → (B ≃ B') → (A + B) ≃ (A' + B')
  pr1 (equiv-coprod e e') = map-equiv-coprod e e'
  pr2 (equiv-coprod e e') =
    is-equiv-map-coprod (is-equiv-map-equiv e) (is-equiv-map-equiv e')
```

### Functoriality of coproducts preserves being surjective

```agda
module _
  {l1 l2 l1' l2' : Level} {A : UU l1} {B : UU l2} {A' : UU l1'} {B' : UU l2'}
  where

  abstract
    is-surjective-map-coprod :
      {f : A → A'} {g : B → B'} →
      is-surjective f → is-surjective g →
      is-surjective (map-coprod f g)
    is-surjective-map-coprod s s' (inl x) =
      apply-universal-property-trunc-Prop (s x)
        ( trunc-Prop (fib (map-coprod _ _) (inl x)))
        ( λ {(a , p) → unit-trunc-Prop (inl a , ap inl p)})
    is-surjective-map-coprod s s' (inr x) =
      apply-universal-property-trunc-Prop (s' x)
        ( trunc-Prop (fib (map-coprod _ _) (inr x)))
        ( λ {(a , p) → unit-trunc-Prop (inr a , ap inr p)})
```

### For any two maps `f : A → B` and `g : C → D`, there is at most one pair of maps `f' : A → B` and `g' : C → D` such that `f' + g' = f + g`

```agda
is-contr-fib-map-coprod :
  {l1 l2 l3 l4 : Level} {A : UU l1} {B : UU l2} {C : UU l3} {D : UU l4}
  (f : A → B) (g : C → D) →
  is-contr
    ( fib ( λ (fg' : (A → B) × (C → D)) → map-coprod (pr1 fg') (pr2 fg'))
          ( map-coprod f g))
is-contr-fib-map-coprod {A = A} {B} {C} {D} f g =
  is-contr-equiv
    ( Σ ( (A → B) × (C → D))
        ( λ fg' →
          ((a : A) → pr1 fg' a ＝ f a) × ((c : C) → pr2 fg' c ＝ g c)))
    ( equiv-tot
      ( λ fg' →
        ( ( equiv-prod
            ( equiv-map-Π
              ( λ a → compute-eq-coprod-inl-inl (pr1 fg' a) (f a)))
            ( equiv-map-Π
              ( λ c → compute-eq-coprod-inr-inr (pr2 fg' c) (g c)))) ∘e
          ( equiv-dependent-universal-property-coprod
            ( λ x →
              map-coprod (pr1 fg') (pr2 fg') x ＝ map-coprod f g x))) ∘e
        ( equiv-funext)))
    ( is-contr-total-Eq-structure
      ( λ f' g' (H : f' ~ f) → (c : C) → g' c ＝ g c)
      ( is-contr-total-htpy' f)
      ( pair f refl-htpy)
      ( is-contr-total-htpy' g))

{-
is-emb-map-coprod :
  {l1 l2 l3 l4 : Level} {A : UU l1} {B : UU l2} {C : UU l3} {D : UU l4} →
  is-emb (λ (fg : (A → B) × (C → D)) → map-coprod (pr1 fg) (pr2 fg))
is-emb-map-coprod (pair f g) =
  fundamental-theorem-id (pair f g)
    ( refl)
    {! is-contr-fib-map-coprod f g!}
    {!!}
-}
```

### For any equivalence `f : A + B ≃ A + B` and `g : B ≃ B` such that `f` and `g` coincide on `B`, we construct an `h : A ≃ A` such that `htpy-equiv (equiv-coprod h d) f`

```agda
module _
  {l1 l2 : Level} {A : UU l1} {B : UU l2}
  where

  equiv-coproduct-induce-equiv-disjoint :
    (f : (A + B) ≃ (A + B)) (g : B ≃ B)
    (p : (b : B) → map-equiv f (inr b) ＝ inr (map-equiv g b))
    (x : A) (y : B) → ¬ (map-equiv f (inl x) ＝ inr y)
  equiv-coproduct-induce-equiv-disjoint f g p x y q =
    neq-inr-inl
      ( is-injective-map-equiv f
        ( ( p (map-equiv (inv-equiv g) y) ∙
          ( ( ap (λ z → inr (map-equiv z y)) (right-inverse-law-equiv g)) ∙
            ( inv q)))))

  inv-commutative-square-inr :
    (f : (A + B) ≃ (A + B)) (g : B ≃ B)
    (p : (b : B) → map-equiv f (inr b) ＝ inr (map-equiv g b)) →
    (b : B) → map-inv-equiv f (inr b) ＝ inr (map-inv-equiv g b)
  inv-commutative-square-inr f g p b =
    is-injective-map-equiv f
      ( ( ap (λ z → map-equiv z (inr b)) (right-inverse-law-equiv f)) ∙
        ( ( inv (ap (λ z → inr (map-equiv z b)) (right-inverse-law-equiv g))) ∙
          ( inv (p (map-inv-equiv g b)))))

  cases-retraction-equiv-coprod :
    (f : (A + B) ≃ (A + B)) (g : B ≃ B)
    (p : (b : B) → map-equiv f (inr b) ＝ inr (map-equiv g b))
    (x : A) (y : A + B) → map-equiv f (inl x) ＝ y → A
  cases-retraction-equiv-coprod f g p x (inl y) q = y
  cases-retraction-equiv-coprod f g p x (inr y) q =
    ex-falso (equiv-coproduct-induce-equiv-disjoint f g p x y q)

  inv-cases-retraction-equiv-coprod :
    (f : (A + B) ≃ (A + B)) (g : B ≃ B)
    (p : (b : B) → map-equiv f (inr b) ＝ inr (map-equiv g b))
    (x : A) (y : A + B) → map-inv-equiv f (inl x) ＝ y → A
  inv-cases-retraction-equiv-coprod f g p =
    cases-retraction-equiv-coprod
      ( inv-equiv f)
      ( inv-equiv g)
      ( inv-commutative-square-inr f g p)

  retraction-cases-retraction-equiv-coprod :
    ( f : (A + B) ≃ (A + B)) (g : B ≃ B)
    ( p : (b : B) → map-equiv f (inr b) ＝ inr (map-equiv g b))
    ( x : A) (y z : A + B) (q : map-equiv f (inl x) ＝ y)
    ( r :
      map-inv-equiv f (inl (cases-retraction-equiv-coprod f g p x y q)) ＝ z) →
    ( inv-cases-retraction-equiv-coprod f g p
      ( cases-retraction-equiv-coprod f g p x y q) z r) ＝
    ( x)
  retraction-cases-retraction-equiv-coprod f g p x (inl y) (inl z) q r =
    is-injective-inl
      ( ( inv r) ∙
        ( ( ap (map-inv-equiv f) (inv q)) ∙
          ( ap (λ w → map-equiv w (inl x)) (left-inverse-law-equiv f))))
  retraction-cases-retraction-equiv-coprod f g p x (inl y) (inr z) q r =
    ex-falso
      ( equiv-coproduct-induce-equiv-disjoint
        ( inv-equiv f)
        ( inv-equiv g)
        ( inv-commutative-square-inr f g p)
        ( y)
        ( z)
        ( r))
  retraction-cases-retraction-equiv-coprod f g p x (inr y) z q r =
    ex-falso (equiv-coproduct-induce-equiv-disjoint f g p x y q)

  section-cases-retraction-equiv-coprod :
    ( f : (A + B) ≃ (A + B)) (g : B ≃ B)
    ( p : (b : B) → map-equiv f (inr b) ＝ inr (map-equiv g b))
    ( x : A) (y z : A + B) (q : map-inv-equiv f (inl x) ＝ y)
    ( r :
      map-equiv f (inl (inv-cases-retraction-equiv-coprod f g p x y q)) ＝ z) →
    ( cases-retraction-equiv-coprod f g p
      ( inv-cases-retraction-equiv-coprod f g p x y q) z r) ＝
    ( x)
  section-cases-retraction-equiv-coprod f g p x (inl y) (inl z) q r =
    is-injective-inl
      ( ( inv r) ∙
        ( ( ap (map-equiv f) (inv q)) ∙
          ( ap (λ w → map-equiv w (inl x)) (right-inverse-law-equiv f))))
  section-cases-retraction-equiv-coprod f g p x (inl y) (inr z) q r =
    ex-falso (equiv-coproduct-induce-equiv-disjoint f g p y z r)
  section-cases-retraction-equiv-coprod f g p x (inr y) z q r =
    ex-falso
      ( equiv-coproduct-induce-equiv-disjoint
        ( inv-equiv f)
        ( inv-equiv g)
        ( inv-commutative-square-inr f g p)
        ( x)
        ( y)
        ( q))

  retraction-equiv-coprod :
    (f : (A + B) ≃ (A + B)) (g : B ≃ B)
    (p : (b : B) → map-equiv f (inr b) ＝ inr (map-equiv g b)) →
    Σ (A ≃ A) (λ h → htpy-equiv f (equiv-coprod h g))
  pr1 (pr1 (retraction-equiv-coprod f g p)) x =
    cases-retraction-equiv-coprod f g p x (map-equiv f (inl x)) refl
  pr2 (pr1 (retraction-equiv-coprod f g p)) =
    is-equiv-has-inverse
      ( λ x →
        inv-cases-retraction-equiv-coprod f g p x
          ( map-inv-equiv f (inl x))
          ( refl))
      ( λ x →
        section-cases-retraction-equiv-coprod f g p x
          ( map-inv-equiv f (inl x))
          ( map-equiv f
            ( inl
              ( inv-cases-retraction-equiv-coprod f g p x
                ( map-inv-equiv f (inl x))
                ( refl))))
          ( refl)
          ( refl))
      ( λ x →
        retraction-cases-retraction-equiv-coprod f g p x
          ( map-equiv f (inl x))
          ( map-inv-equiv f
            ( inl
              ( cases-retraction-equiv-coprod f g p x
                ( map-equiv f (inl x))
                ( refl))))
          ( refl)
          ( refl))
  pr2 (retraction-equiv-coprod f g p) (inl x) =
    commutative-square-inl-retraction-equiv-coprod x (map-equiv f (inl x)) refl
    where
    commutative-square-inl-retraction-equiv-coprod :
      (x : A) (y : A + B) (q : map-equiv f (inl x) ＝ y) →
      map-equiv f (inl x) ＝ inl (cases-retraction-equiv-coprod f g p x y q)
    commutative-square-inl-retraction-equiv-coprod x (inl y) q = q
    commutative-square-inl-retraction-equiv-coprod x (inr y) q =
      ex-falso (equiv-coproduct-induce-equiv-disjoint f g p x y q)
  pr2 (retraction-equiv-coprod f g p) (inr x) = p x
```

### Equivalences between mutually exclusive coproducts

If `P → ¬ Q'` and `P' → ¬ Q` then `(P + Q ≃ P' + Q') ≃ ((P ≃ P') × (Q ≃ Q'))`.

```agda
module _
  {l1 l2 l3 l4 : Level}
  {P : UU l1} {Q : UU l2} {P' : UU l3} {Q' : UU l4}
  (¬PQ' : P → ¬ Q')
  where

  left-to-left :
    (e : (P + Q) ≃ (P' + Q')) →
    (u : P + Q) → is-left u → is-left (map-equiv e u)
  left-to-left e (inl p) _ =
    ind-coprod is-left (λ _ → star) (λ q' → ¬PQ' p q') (map-equiv e (inl p))
  left-to-left e (inr q) ()

module _
  {l1 l2 l3 l4 : Level}
  {P : UU l1} {Q : UU l2} {P' : UU l3} {Q' : UU l4}
  (¬P'Q : P' → ¬ Q)
  where

  right-to-right :
    (e : (P + Q) ≃ (P' + Q')) (u : P + Q) →
    is-right u → is-right (map-equiv e u)
  right-to-right e (inl p) ()
  right-to-right e (inr q) _ =
    ind-coprod is-right (λ p' → ¬P'Q p' q) (λ _ → star) (map-equiv e (inr q))

module _
  {l1 l2 l3 l4 : Level}
  {P : UU l1} {Q : UU l2} {P' : UU l3} {Q' : UU l4}
  (¬PQ' : P → ¬ Q') (¬P'Q : P' → ¬ Q)
  where

  equiv-left-to-left :
    (e : (P + Q) ≃ (P' + Q')) (u : P + Q) → is-left u ≃ is-left (map-equiv e u)
  pr1 (equiv-left-to-left e u) = left-to-left ¬PQ' e u
  pr2 (equiv-left-to-left e u) =
    is-equiv-has-inverse
      ( tr is-left (is-retraction-map-inv-equiv e u) ∘
        left-to-left ¬P'Q (inv-equiv e) (map-equiv e u))
      ( λ _ → eq-is-prop (is-prop-is-left (map-equiv e u)))
      ( λ _ → eq-is-prop (is-prop-is-left u))

  equiv-right-to-right :
    (e : (P + Q) ≃ (P' + Q')) (u : P + Q) →
    is-right u ≃ is-right (map-equiv e u)
  pr1 (equiv-right-to-right e u) = right-to-right ¬P'Q e u
  pr2 (equiv-right-to-right e u) =
    is-equiv-has-inverse
      ( tr is-right (is-retraction-map-inv-equiv e u) ∘
        right-to-right ¬PQ' (inv-equiv e) (map-equiv e u))
      (λ _ → eq-is-prop (is-prop-is-right (map-equiv e u)))
      (λ _ → eq-is-prop (is-prop-is-right u))

  map-mutually-exclusive-coprod : (P + Q) ≃ (P' + Q') → (P ≃ P') × (Q ≃ Q')
  pr1 (map-mutually-exclusive-coprod e) =
    equiv-left-summand ∘e
    ( equiv-Σ _ e (equiv-left-to-left e) ∘e
      inv-equiv equiv-left-summand)
  pr2 (map-mutually-exclusive-coprod e) =
    equiv-right-summand ∘e
    ( equiv-Σ _ e (equiv-right-to-right e) ∘e
      inv-equiv (equiv-right-summand))

  map-inv-mutually-exclusive-coprod : (P ≃ P') × (Q ≃ Q') → (P + Q) ≃ (P' + Q')
  map-inv-mutually-exclusive-coprod (pair e₁ e₂) = equiv-coprod e₁ e₂

  is-retraction-map-inv-mutually-exclusive-coprod :
    (map-mutually-exclusive-coprod ∘ map-inv-mutually-exclusive-coprod) ~ id
  is-retraction-map-inv-mutually-exclusive-coprod (pair e₁ e₂) =
    eq-pair
      (eq-equiv-eq-map-equiv refl)
      (eq-equiv-eq-map-equiv refl)

  is-section-map-inv-mutually-exclusive-coprod :
    (map-inv-mutually-exclusive-coprod ∘ map-mutually-exclusive-coprod) ~ id
  is-section-map-inv-mutually-exclusive-coprod e =
    eq-htpy-equiv (
      λ { (inl p) →
          ap
            ( pr1)
            ( is-retraction-map-inv-equiv-left-summand
              ( map-equiv e (inl p) , left-to-left ¬PQ' e (inl p) star)) ;
          (inr q) →
          ap
            ( pr1)
            ( is-retraction-map-inv-equiv-right-summand
              ( map-equiv e (inr q) , right-to-right ¬P'Q e (inr q) star))})

  equiv-mutually-exclusive-coprod :
    ((P + Q) ≃ (P' + Q')) ≃ ((P ≃ P') × (Q ≃ Q'))
  pr1 equiv-mutually-exclusive-coprod = map-mutually-exclusive-coprod
  pr2 equiv-mutually-exclusive-coprod =
    is-equiv-has-inverse
      map-inv-mutually-exclusive-coprod
      is-retraction-map-inv-mutually-exclusive-coprod
      is-section-map-inv-mutually-exclusive-coprod
```

## See also

- Arithmetical laws involving coproduct types are recorded in
  [`foundation.type-arithmetic-coproduct-types`](foundation.type-arithmetic-coproduct-types.md).
- Equality proofs in coproduct types are characterized in
  [`foundation.equality-coproduct-types`](foundation.equality-coproduct-types.md).
- The universal property of coproducts is treated in
  [`foundation.universal-property-coproduct-types`](foundation.universal-property-coproduct-types.md).

- Functorial properties of cartesian product types are recorded in
  [`foundation.functoriality-cartesian-product-types`](foundation.functoriality-cartesian-product-types.md).
- Functorial properties of dependent pair types are recorded in
  [`foundation.functoriality-dependent-pair-types`](foundation.functoriality-dependent-pair-types.md).
